Foundation/Modal/Boxdot/GL_Grz.lean
@@ -8,33 +8,15 @@ namespace Kripke
 open Relation (ReflGen)
 open Formula.Kripke
 
+variable {F : Frame} {φ : Formula _}
+
 lemma mem_reflClosure_GrzFiniteFrameClass_of_mem_GLFiniteFrameClass (hF : F ∈ FrameClass.finite_trans_irrefl) : F^= ∈ FrameClass.finite_partial_order := by
-  obtain ⟨_, F_trans, F_irrefl⟩ := hF;
-  refine ⟨inferInstance, ?F_refl, ?F_trans, ?F_antisymm⟩;
-  . intro x; apply ReflGen.refl;
-  . rintro x y z (rfl | Rxy) (rfl | Ryz);
-    . apply ReflGen.refl;
-    . apply ReflGen.single Ryz;
-    . apply ReflGen.single Rxy;
-    . apply ReflGen.single $ F_trans Rxy Ryz;
-  . rintro x y (rfl | Rxy) (rfl | Ryx);
-    . rfl;
-    . rfl;
-    . rfl;
-    . have := F_trans Rxy Ryx;
-      have := F_irrefl x;
-      contradiction;
+  obtain ⟨_, _, _⟩ := hF;
+  refine ⟨inferInstance, inferInstance⟩;
 
 lemma mem_irreflClosure_GLFiniteFrameClass_of_mem_GrzFiniteFrameClass (hF : F ∈ FrameClass.finite_partial_order) : F^≠ ∈ FrameClass.finite_trans_irrefl := by
   obtain ⟨_, _, F_trans, F_antisymm⟩ := hF;
-  refine ⟨inferInstance, ?F_trans, ?F_irrefl⟩;
-  . rintro x y z ⟨nexy, Rxy⟩ ⟨_, Ryz⟩;
-    constructor;
-    . by_contra; subst_vars;
-      have := F_antisymm Rxy Ryz;
-      contradiction;
-    . exact F_trans Rxy Ryz;
-  . exact Frame.mkIrreflClosure.rel_irreflexive;
+  refine ⟨inferInstance, inferInstance, inferInstance⟩;
 
 lemma iff_boxdot_reflexive_closure : (Satisfies ⟨F, V⟩ x (φᵇ)) ↔ (Satisfies ⟨F^=, V⟩ x φ) := by
   induction φ using Formula.rec' generalizing x with
@@ -62,12 +44,12 @@ lemma iff_boxdot_reflexive_closure : (Satisfies ⟨F, V⟩ x (φᵇ)) ↔ (Satis
         exact @h y (ReflGen.single Rxy);
   | _ => rfl;
 
-lemma iff_frame_boxdot_reflexive_closure {F : Frame} : (F ⊧ (φᵇ)) ↔ ((F^=) ⊧ φ) := by
+lemma iff_frame_boxdot_reflexive_closure : (F ⊧ (φᵇ)) ↔ ((F^=) ⊧ φ) := by
   constructor;
   . intro h V x; apply iff_boxdot_reflexive_closure.mp; exact h V x;
   . intro h V x; apply iff_boxdot_reflexive_closure.mpr; exact h V x;
 
-lemma iff_reflexivize_irreflexivize {F : Frame} (F_Refl : Reflexive F) {x : F.World} {V} : (Satisfies ⟨F, V⟩ x φ) ↔ (Satisfies ⟨F^≠^=, V⟩ x φ) := by
+lemma iff_reflexivize_irreflexivize [IsRefl _ F] {x : F.World} {V} : (Satisfies ⟨F, V⟩ x φ) ↔ (Satisfies ⟨F^≠^=, V⟩ x φ) := by
   induction φ using Formula.rec' generalizing x with
   | hatom φ => rfl;
   | hfalsum => rfl;
@@ -85,7 +67,7 @@ lemma iff_reflexivize_irreflexivize {F : Frame} (F_Refl : Reflexive F) {x : F.Wo
       apply ihp (x := y) |>.mp;
       exact h y $ by
         induction Rxy with
-        | refl => apply F_Refl
+        | refl => apply IsRefl.refl;
         | single h => exact h.2;
     . intro h y Rxy;
       by_cases e : x = y;
@@ -95,6 +77,11 @@ lemma iff_reflexivize_irreflexivize {F : Frame} (F_Refl : Reflexive F) {x : F.Wo
       . apply ihp (x := y) |>.mpr;
         exact h y $ by
           exact ReflGen.single ⟨(by simpa), Rxy⟩;
+
+lemma iff_reflexivize_irreflexivize' [IsRefl _ F] : (F ⊧ φ) ↔ ((F^≠^=) ⊧ φ) := by
+  constructor;
+  . intro h V x; apply iff_reflexivize_irreflexivize.mp; exact h V x;
+  . intro h V x; apply iff_reflexivize_irreflexivize.mpr; exact h V x;
 
 end Kripke
 
@@ -117,24 +104,15 @@ lemma provable_boxdotTranslated_GL_of_Grz : (Hilbert.Grz) ⊢! φ → (Hilbert.G
 lemma provable_Grz_of_boxdotTranslated_GL : (Hilbert.GL) ⊢! φᵇ → (Hilbert.Grz) ⊢! φ := by
   contrapose;
   intro h;
-  obtain ⟨F, ⟨_, F_refl, F_trans, F_antisymm⟩, h⟩ := iff_not_validOnFrameClass_exists_frame.mp $ (not_imp_not.mpr $ Hilbert.Grz.Kripke.complete |>.complete) h;
+  obtain ⟨F, ⟨_, _, _⟩, h⟩ := iff_not_validOnFrameClass_exists_frame.mp $ (not_imp_not.mpr $ Hilbert.Grz.Kripke.complete |>.complete) h;
   apply not_imp_not.mpr $ Hilbert.GL.Kripke.finite_sound.sound;
   apply iff_not_validOnFrameClass_exists_frame.mpr;
   use F^≠;
   constructor;
-  . suffices Transitive (F^≠).Rel by refine ⟨inferInstance, by assumption, Frame.mkIrreflClosure.rel_irreflexive⟩;
-    rintro x y z ⟨hxy, Rxy⟩ ⟨hyz, Ryz⟩;
-    constructor;
-    . by_contra hC;
-      subst hC;
-      have := F_antisymm Rxy Ryz;
-      contradiction;
-    . exact F_trans Rxy Ryz;
+  . refine ⟨inferInstance, inferInstance, inferInstance⟩;
   . apply Kripke.iff_frame_boxdot_reflexive_closure.not.mpr;
-    apply Formula.Kripke.ValidOnFrame.not_of_exists_valuation_world;
-    obtain ⟨V, x, hx⟩ := Formula.Kripke.ValidOnFrame.iff_not_exists_valuation_world.mp h;
-    use V, x;
-    exact iff_reflexivize_irreflexivize F_refl |>.not.mp hx;
+    apply iff_reflexivize_irreflexivize'.not.mp;
+    exact h;
 
 theorem iff_boxdotTranslatedGL_Grz : (Hilbert.GL) ⊢! φᵇ ↔ (Hilbert.Grz) ⊢! φ := ⟨
   provable_Grz_of_boxdotTranslated_GL,
