Foundation/Modal/Kripke/Hilbert/Triv.lean
@@ -10,17 +10,15 @@ open Geachean
 protected abbrev Kripke.FrameClass.refl_corefl : FrameClass := { F | IsRefl _ F ∧ IsCoreflexive _ F }
 protected abbrev Kripke.FrameClass.equality : FrameClass := { F | IsEquality _ F }
 
-/-
 lemma Kripke.FrameClass.eq_equality_refl_corefl : Kripke.FrameClass.equality = Kripke.FrameClass.refl_corefl := by
   ext F;
   constructor;
-  . intro hEq;
-    constructor;
-    . exact refl_of_equality hEq;
-    . exact corefl_of_equality hEq;
+  . intro F_eq;
+    replace F_eq := Set.mem_setOf_eq.mp F_eq;
+    constructor <;> infer_instance;
   . rintro ⟨hRefl, hCorefl⟩;
-    exact equality_of_refl_corefl hRefl hCorefl;
--/
+    apply Set.mem_setOf_eq.mpr;
+    infer_instance;
 
 namespace Hilbert.Triv.Kripke
 
@@ -31,11 +29,9 @@ instance sound_refl_corefl : Sound (Hilbert.Triv) Kripke.FrameClass.refl_corefl 
     . exact validate_AxiomT_of_reflexive;
     . exact validate_AxiomTc_of_coreflexive;
 
-/-
 instance sound_equality : Sound (Hilbert.Triv) Kripke.FrameClass.equality := by
   rw [Kripke.FrameClass.eq_equality_refl_corefl];
-  exact Kripke.sound_refl_corefl;
--/
+  infer_instance;
 
 instance consistent : Entailment.Consistent (Hilbert.Triv) := consistent_of_sound_frameclass Kripke.FrameClass.refl_corefl $ by
   use whitepoint;
@@ -48,11 +44,9 @@ instance cannonical_refl_corefl : Canonical (Hilbert.Triv) Kripke.FrameClass.ref
 
 instance complete_refl_corefl : Complete (Hilbert.Triv) Kripke.FrameClass.refl_corefl := inferInstance
 
-/-
 instance complete_equality : Complete (Hilbert.Triv) Kripke.FrameClass.equality := by
   rw [Kripke.FrameClass.eq_equality_refl_corefl];
-  exact Kripke.complete_refl_corefl;
--/
+  infer_instance;
 
 end Hilbert.Triv.Kripke
 
