Foundation/Modal/Logic/Sublogic/KTc.lean
@@ -17,16 +17,18 @@ instance : ProperSublogic Logic.KTc Logic.Triv := ⟨by
     . apply Kripke.not_validOnFrameClass_of_exists_model_world;
       use ⟨⟨Fin 2, λ x y => False⟩, λ w _ => False⟩, 0;
       constructor;
-      . simp [Coreflexive];
+      . refine ⟨by tauto⟩;
       . simp [Satisfies, Semantics.Realize];
 ⟩
 
 instance : ProperSublogic Logic.KTc Logic.Ver := ⟨by
   constructor;
   . rw [KTc.eq_CoreflexiveKripkeFrameClass_Logic, Ver.eq_IsolatedFrameClass_Logic];
-    rintro φ hφ F F_iso;
+    rintro φ hφ F hF;
+    replace hF := Set.mem_setOf_eq.mp hF;
     apply hφ;
-    simp_all [Coreflexive, Isolated];
+    apply Set.mem_setOf_eq.mpr;
+    infer_instance;
   . suffices ∃ φ, Hilbert.Ver ⊢! φ ∧ ¬FrameClass.corefl ⊧ φ by
       simpa [KTc.eq_CoreflexiveKripkeFrameClass_Logic];
     use (Axioms.Ver ⊥);
@@ -36,7 +38,7 @@ instance : ProperSublogic Logic.KTc Logic.Ver := ⟨by
       let M : Model := ⟨⟨Fin 1, λ x y => True⟩, λ w _ => False⟩;
       use M, 0;
       constructor;
-      . simp [M, Coreflexive]; aesop;
+      . refine ⟨by unfold Coreflexive; trivial⟩
       . suffices ∃ x, (0 : M.World) ≺ x by simpa [Satisfies, Semantics.Realize];
         use 0;
 ⟩
@@ -45,14 +47,9 @@ instance : ProperSublogic Logic.KB4 Logic.KTc := ⟨by
   constructor;
   . rw [KB4.eq_ReflexiveTransitiveKripkeFrameClass_Logic, KTc.eq_CoreflexiveKripkeFrameClass_Logic];
     rintro φ hφ F F_corefl;
+    replace hF := Set.mem_setOf_eq.mp F_corefl;
     apply hφ;
-    refine ⟨?_, ?_⟩;
-    . intro x y Rxy;
-      rw [F_corefl Rxy] at *;
-      assumption;
-    . intro x y z Rxy Ryz;
-      rw [F_corefl Rxy, F_corefl Ryz] at *;
-      assumption;
+    refine ⟨inferInstance, inferInstance⟩;
   . suffices ∃ φ, Hilbert.KTc ⊢! φ ∧ ¬Kripke.FrameClass.symm_trans ⊧ φ by
       simpa [KB4.eq_ReflexiveTransitiveKripkeFrameClass_Logic];
     use (Axioms.Tc (.atom 0));
@@ -62,7 +59,7 @@ instance : ProperSublogic Logic.KB4 Logic.KTc := ⟨by
       let M : Model := ⟨⟨Fin 2, λ x y => True⟩, λ w _ => w = 0⟩;
       use M, 0;
       constructor;
-      . simp [Symmetric, Transitive, M];
+      . refine ⟨⟨by simp [M]⟩, ⟨by simp [M]⟩⟩
       . suffices ∃ x, (x : M.World) ≠ 0 by
           simp [M, Semantics.Realize, Satisfies];
           tauto;
