Foundation/Modal/Logic/Sublogic/S4.lean
@@ -17,10 +17,8 @@ theorem S4_ssubset_S4Point2 : Logic.S4 ⊂ Logic.S4Point2 := by
       let M : Model := ⟨⟨Fin 3, λ x y => (x = 0) ∨ (x = y) ⟩, λ w _ => w = 1⟩;
       use M, 0;
       constructor;
-      . constructor;
-        . simp [M, Reflexive];
-        . unfold Transitive;
-          omega;
+      . apply isPreorder_iff _ _ |>.mpr;
+        refine ⟨⟨?_⟩, ⟨?_⟩⟩ <;> omega;
       . suffices ∃ x, (0 : M.World) ≺ x ∧ (∀ y, x ≺ y → y = 1) ∧ ∃ x, (0 : M.World) ≺ x ∧ ¬x ≺ 1 by
           simpa [M, Semantics.Realize, Satisfies];
         use 1;
@@ -40,25 +38,25 @@ instance : ProperSublogic Logic.S4 Logic.S4Point2 := ⟨S4_ssubset_S4Point2⟩
 theorem S4Point2_ssubset_S4Point3 : Logic.S4Point2 ⊂ Logic.S4Point3 := by
   constructor;
   . rw [S4Point2.eq_ReflexiveTransitiveConfluentKripkeFrameClass_Logic, S4Point3.eq_ReflexiveTransitiveConnectedKripkeFrameClass_Logic];
-    rintro φ hφ F ⟨F_refl, F_trans, F_conn⟩;
+    rintro φ hφ F ⟨_, _⟩;
     apply hφ;
-    refine ⟨?_, ?_, ?_⟩;
-    . exact F_refl;
-    . exact F_trans;
-    . exact confluent_of_refl_connected F_refl F_conn;
+    refine ⟨inferInstance, inferInstance⟩;
   . suffices ∃ φ, Hilbert.S4Point3 ⊢! φ ∧ ¬FrameClass.confluent_preorder ⊧ φ by
       simpa [S4Point2.eq_ReflexiveTransitiveConfluentKripkeFrameClass_Logic];
     use Axioms.Point3 (.atom 0) (.atom 1);
     constructor;
     . exact axiomPoint3!;
     . apply Kripke.not_validOnFrameClass_of_exists_model_world;
-      let M : Model := ⟨⟨Fin 4, λ x y => ¬(x = 1 ∧ y = 2) ∧ ¬(x = 2 ∧ y = 1) ∧ (x ≤ y)⟩, λ w a => (a = 0 ∧ (w = 1 ∨ w = 3)) ∨ (a = 1 ∧ (w = 2 ∨ w = 3))⟩;
+      let M : Model := ⟨
+        ⟨Fin 4, λ x y => ¬(x = 1 ∧ y = 2) ∧ ¬(x = 2 ∧ y = 1) ∧ (x ≤ y)⟩,
+        λ w a => (a = 0 ∧ (w = 1 ∨ w = 3)) ∨ (a = 1 ∧ (w = 2 ∨ w = 3))
+      ⟩;
       use M, 0;
       constructor;
-      . simp only [Set.mem_setOf_eq];
-        refine ⟨?_, ?_, ?_⟩;
-        . simp [M, Reflexive]; omega;
-        . simp [M, Transitive]; omega;
+      . apply Set.mem_setOf_eq.mpr
+        refine ⟨?_, ⟨?_⟩⟩;
+        . apply isPreorder_iff _ _ |>.mpr;
+          refine ⟨⟨by omega⟩, ⟨by omega⟩⟩;
         . rintro x y z ⟨Rxy, Ryz⟩;
           use 3;
           constructor <;> omega;
@@ -86,11 +84,9 @@ theorem S4Point3_ssubset_S5 : Logic.S4Point3 ⊂ Logic.S5 := by
   constructor;
   . rw [S4Point3.eq_ReflexiveTransitiveConnectedKripkeFrameClass_Logic, S5.eq_UniversalKripkeFrameClass_Logic];
     rintro φ hφ F F_univ;
+    replace F_univ := Set.mem_setOf_eq.mp F_univ
     apply hφ;
-    refine ⟨?_, ?_, ?_⟩;
-    . unfold Reflexive; intros; apply F_univ;
-    . unfold Transitive; intros; apply F_univ;
-    . unfold Connected; intros; constructor; apply F_univ;
+    refine ⟨inferInstance, inferInstance⟩;
   . suffices ∃ φ, Hilbert.S5 ⊢! φ ∧ ¬FrameClass.connected_preorder ⊧ φ by
       simpa [S4Point3.eq_ReflexiveTransitiveConnectedKripkeFrameClass_Logic];
     use Axioms.Five (.atom 0);
@@ -100,10 +96,10 @@ theorem S4Point3_ssubset_S5 : Logic.S4Point3 ⊂ Logic.S5 := by
       let M : Model := ⟨⟨Fin 2, λ x y => x ≤ y⟩, λ w a => (w = 0)⟩;
       use M, 0;
       constructor;
-      . simp only [Set.mem_setOf_eq];
-        refine ⟨?_, ?_, ?_⟩;
-        . simp [M, Reflexive];
-        . simp [M, Transitive]; omega;
+      . apply Set.mem_setOf_eq.mpr;
+        refine ⟨?_, ⟨?_⟩⟩;
+        . apply isPreorder_iff _ _ |>.mpr;
+          refine ⟨⟨by omega⟩, ⟨by omega⟩⟩;
         . rintro x y z ⟨Rxy, Ryz⟩; omega;
       . suffices (0 : M.World) ≺ 0 ∧ ∃ x, (0 : M.World) ≺ x ∧ ¬x ≺ 0 by
           simpa [M, Semantics.Realize, Satisfies];
