Foundation/Vorspiel/Relation/Closure.lean
@@ -1,8 +1,35 @@
 import Mathlib.Logic.Relation
+import Mathlib.Tactic.ByContra
 
 namespace Relation
 
 variable {α} {r : α → α → Prop}
+
+
+namespace ReflGen
+
+instance : IsRefl α (ReflGen r) := ⟨by apply ReflGen.refl⟩
+
+instance [IsTrans _ r] : IsTrans α (ReflGen r) := ⟨by
+  rintro a b c (rfl | Rab) (rfl | Rbc);
+  . exact ReflGen.refl;
+  . exact ReflGen.single Rbc;
+  . exact ReflGen.single Rab;
+  . exact ReflGen.single $ IsTrans.trans a b c Rab Rbc;
+⟩
+
+instance [IsIrrefl _ r] [IsTrans _ r] : IsAntisymm α (ReflGen r) := ⟨by
+  rintro a b (rfl | Rab) (rfl | Rba);
+  . trivial;
+  . trivial;
+  . trivial;
+  . exfalso;
+    exact IsIrrefl.irrefl a $ IsTrans.trans a b a Rab Rba
+⟩
+
+instance [IsTrans _ r] [IsIrrefl _ r] : IsPartialOrder α (ReflGen r) where
+
+end ReflGen
 
 
 namespace TransGen
@@ -12,12 +39,20 @@ instance : IsTrans α (TransGen r) := ⟨by apply TransGen.trans⟩
 end TransGen
 
 
-
 section Irrefl
 
 def IrreflGen (r : α → α → Prop) := λ x y => x ≠ y ∧ r x y
 
 instance : IsIrrefl α (IrreflGen r) := ⟨by simp [IrreflGen]⟩
+
+instance [IsTrans α r] [IsAntisymm α r] : IsTrans α (IrreflGen r) := ⟨by
+  rintro a b c ⟨hne, Rab⟩ ⟨_, Rbc⟩;
+  constructor;
+  . by_contra hC;
+    subst hC;
+    exact hne $ IsAntisymm.antisymm a b Rab Rbc;
+  . exact IsTrans.trans a b c Rab Rbc;
+⟩
 
 end Irrefl
 
